Refactoring the correctness theorem and the trace similarity thms in response to the changes made in the H-VHDL semantics.

behavior-preservation/SemanticPreservation.v
@@ -1,4 +1,4 @@
-(** * Semantic Preservation Theorem *)
+(** * Semantic preservation theorem *)
 
 Require Import NatMap.
 
@@ -22,14 +22,13 @@ Require Import hvhdl.HVhdlTypes.
 Require Import hvhdl.Environment.
 Require Import hvhdl.SemanticalDomains.
 Require Import hvhdl.Simulation.
-Require Import hvhdl.CombinationalEvaluation.
-Require Import hvhdl.SynchronousEvaluation.
 Require Import hvhdl.DesignElaboration.
 Require Import hvhdl.AbstractSyntax.
 Require Import hvhdl.HilecopDesignStore.
 Require Import hvhdl.Initialization.
-Require Import hvhdl.Stabilize.
+Require Import hvhdl.Stabilization.
 Require Import hvhdl.PortMapEvaluation.
+Require Import hvhdl.TypeElaboration.
 
 (* SITPN to H-VHDL Libraries *)
 
@@ -39,6 +38,7 @@ Require Import transformation.GenerateHVhdl.
 
 Require Import soundness.SemanticPreservationDefs.
 Require Import soundness.TraceSimilarity.
+
 (* Require Import soundness.InitialStates. *)
 (* Require Import soundness.RisingEdge. *)
 (* Require Import soundness.FallingEdge. *)
@@ -53,13 +53,13 @@ Local Unset Implicit Arguments.
     SITPN model [sitpn]. *)
 
 Axiom sitpn2hvhdl_elab_ex :
-  forall sitpn id__ent id__arch mm d γ,
+  forall sitpn b d γ,
 
     (* The SITPN model [sitpn] is well-defined. *)
     IsWellDefined sitpn ->
     
     (* sitpn translates into (d, γ). *)
-    sitpn2hvhdl sitpn id__ent id__arch mm = (inl (d, γ)) ->
+    sitpn2hvhdl sitpn b = (inl (d, γ)) ->
 
     (* there exists an elaborated version [Δ] of [d], with a default state [σ__e] *)
     exists Δ σ__e, EDesign hdstore (NatMap.empty value) d Δ σ__e.
@@ -72,82 +72,100 @@ Axiom sitpn2hvhdl_elab_ex :
     default design state [σ__e].  *)
 
 Axiom sitpn2vhdl_init_state_ex :
-  forall sitpn id__ent id__arch mm d γ Δ σ__e,
+  forall sitpn b d γ Δ σ__e,
 
     (* The SITPN model [sitpn] is well-defined. *)
     IsWellDefined sitpn ->
     
     (* sitpn translates into (d, γ). *)
-    sitpn2hvhdl sitpn id__ent id__arch mm = (inl (d, γ)) ->
+    sitpn2hvhdl sitpn b = (inl (d, γ)) ->
 
     (* An elaborated version [Δ] of [d], with a default state [σ__e] *)
     EDesign hdstore (NatMap.empty value) d Δ σ__e ->
 
     (* There exists an initial state [σ0] of [d]. *)
-    exists σ0, Init hdstore Δ σ__e (behavior d) σ0. 
+    exists σ0, Init hdstore Δ σ__e (beh d) σ0. 
 
 (** ** Simulation trace theorem *)
 
-(** The simulation environment [E__p] is well-defined, i.e, it
-    associates a value of the right type to all the input ports of
-    [Δ]. *)
+(** The simulation environment [E__p] is well-defined, i.e. at each time
+    count, it associates a value of the right type to all the
+    identifiers declared as input ports of the design [d].  *)
 
-Definition IsWellDefinedSimEnv (Δ : ElDesign) (E__p : nat -> IdMap value) : Prop :=
-  forall τ,
-    (forall id v, MapsTo id v (E__p τ) -> exists t, MapsTo id (Input t) Δ /\ IsOfType v t)
-    /\ (forall id t, MapsTo id (Input t) Δ -> exists v, MapsTo id v (E__p τ) /\ IsOfType v t).
+Definition IsWDSimEnvForDesign (d : design) (E__p : nat -> IdMap value) : Prop :=
+  forall tc,
+    (forall id v, MapsTo id v (E__p tc) -> exists τ, In (pdecl_in id τ) (ports d) /\ forall Δ t, EType Δ τ t -> IsOfType v t).
 
-Axiom IsWellDefinedSimEnv_ex :
-  forall Δ, exists E__p, IsWellDefinedSimEnv Δ E__p.
+(** The simulation environment [E__p] is well-defined, i.e. it
+    associates a value of the right type to all the input ports
+    declared in the elaborated design [Δ]. Injectivity of the map
+    yielded by the [E__p] function at a given time count [τ] regarding
+    the set of input port identifiers declared in [Δ]. *)
 
-Axiom SimEnv_ex : forall sitpn γ E__c, exists E__p, SimEnv sitpn γ E__c E__p.
+Definition IsWDSimEnvForElDesign (Δ : ElDesign) (E__p : nat -> IdMap value) : Prop :=
+  forall tc,
+    (forall id v, MapsTo id v (E__p tc) -> exists t, MapsTo id (Input t) Δ /\ IsOfType v t).
+
+(** States that if an simulation environment [E__p] is well-defined for
+    a design [d], then it is well-defined for the elaborated version
+    of the design [Δ]. *)
+
+Lemma IsWDSimEnv_trans :
+  forall D__s M__g d Δ σ__e,
+    EDesign D__s M__g d Δ σ__e ->
+    forall E__p,
+      IsWDSimEnvForDesign d E__p -> IsWDSimEnvForElDesign Δ E__p.
+Admitted.
 
 (** There exist a simulation trace [θ__σ] that verify the [SimLoop] for
     all design [d] result of the transformation of a well-defined and
     bounded SITPN model [sitpn]. *)
 
 Axiom sitpn2vhdl_sim_ex :
-  forall sitpn id__ent id__arch mm d γ Δ σ__e σ0 τ E__p b,
+  forall sitpn (b : P sitpn -> nat) d γ Δ σ__e σ0 τ E__p b,
 
     (* The SITPN model [sitpn] is well-defined. *)
     IsWellDefined sitpn ->
 
     (* The SITPN model [sitpn] is bounded through [b]. *)
-    @BoundedSitpn sitpn b ->
+    BoundedSitpn b ->
     
     (* sitpn translates into (d, γ). *)
-    sitpn2hvhdl sitpn id__ent id__arch mm = (inl (d, γ)) ->
+    sitpn2hvhdl sitpn b = (inl (d, γ)) ->
 
     (* An elaborated version [Δ] of [d], with a default state [σ__e] *)
     EDesign hdstore (NatMap.empty value) d Δ σ__e ->
 
     (* An initial state [σ0] of [d]. *)
-    Init hdstore Δ σ__e (behavior d) σ0 ->
+    Init hdstore Δ σ__e (beh d) σ0 ->
 
     (* The simulation env [E__p] is well-defined. *)
-    IsWellDefinedSimEnv Δ E__p ->
+    IsWDSimEnvForElDesign Δ E__p ->
     
-    exists θ__σ, SimLoop hdstore E__p Δ σ0 (behavior d) τ θ__σ.
+    exists θ__σ, SimLoop hdstore E__p Δ σ0 (beh d) τ θ__σ.
 
 (** ** Semantic preservation theorem  *)
 
 Theorem sitpn2vhdl_semantic_preservation :
-  forall sitpn id__ent id__arch b d γ E__c τ θ__s,
+  forall sitpn b d γ E__c τ θ__s,
 
     (* [sitpn] is well-defined. *)
     IsWellDefined sitpn ->
     
     (* [sitpn] is bounded through [b]. *)
-    @BoundedSitpn sitpn b ->
+    BoundedSitpn b ->
     
     (* sitpn translates into (d, γ). *)
-    sitpn2hvhdl sitpn id__ent id__arch b = (inl (d, γ)) ->
+    sitpn2hvhdl sitpn b = (inl (d, γ)) ->
     
     (* SITPN [sitpn] yields execution trace [θ__s] after [τ] execution cycles. *)
     
     @SitpnFullExec sitpn E__c τ θ__s ->    
 
     forall E__p,
+
+      (* [E__p] is a well-defined simulation environment for design [d]. *)
+      IsWDSimEnvForDesign d E__p ->
       
       (* Environments are similar. *)
       SimEnv sitpn γ E__c E__p ->
@@ -160,20 +178,20 @@ Theorem sitpn2vhdl_semantic_preservation :
         (* Traces are fully similar. *)
         FullSimTrace γ θ__s θ__σ.
 Proof.
-  (* intros. *)
-  (* edestruct sitpn2hvhdl_elab_ex as (Δ, (σ__e, Helab)); eauto. *)
-  (* edestruct sitpn2vhdl_init_state_ex as (σ0, Hinit); eauto. *)
-  (* exists Δ; intros. *)
-  (* edestruct @sitpn2vhdl_sim_ex with (τ := τ) as (θ__σ, Hsim); eauto.   *)
-  (* exists (σ0 :: θ__σ). split. *)
+  intros.
+  edestruct sitpn2hvhdl_elab_ex as (Δ, (σ__e, Helab)); eauto.
+  edestruct sitpn2vhdl_init_state_ex as (σ0, Hinit); eauto.
+  edestruct @sitpn2vhdl_sim_ex with (τ := τ) as (θ__σ, Hsim); eauto.
+  eapply IsWDSimEnv_trans; eauto.
+  exists (σ0 :: θ__σ). split.
 
-  (* Existence of an elaborated design [Δ], a default state [σ__e], an
-     initial state [σ0], and a simulation trace [θ__σ]. *)
-  (* unfold HFullSim; eapply FullSim; eauto. *)
+  (* Existence of an elaborated design [Δ], a default state [σ__e], an *)
+  (*    initial state [σ0], and a simulation trace [θ__σ]. *)
+  unfold HFullSim; eapply FullSim_; eauto.
 
   (* Similar traces. *)
-  (* eapply trace_sim; eauto. *)
-  (* unfold HFullSim; eapply FullSim; eauto.   *)
+  eapply trace_sim; eauto.
+  unfold HFullSim; eapply FullSim; eauto.
 Admitted.
 
 
