behavior-preservation/FirstRisingEdge.v
@@ -12,10 +12,10 @@ Require Import transformation.Sitpn2HVhdl.
 Require Import soundness.SemanticPreservationDefs.
 
 Lemma first_rising_edge_full :
-  forall sitpn id__ent id__arch b d γ E__c E__p Δ σ__e σ0 τ σ__i σ__r σ,
+  forall sitpn b d γ E__c E__p Δ σ__e σ0 τ σ__r σ,
 
     (* sitpn translates into (d, γ). *)
-    sitpn2hvhdl sitpn id__ent id__arch b = (inl (d, γ)) ->
+    sitpn2hvhdl sitpn b = (inl (d, γ)) ->
 
     (* Environments are similar. *)
     SimEnv sitpn γ E__c E__p ->
@@ -24,12 +24,11 @@ Lemma first_rising_edge_full :
     EDesign hdstore (NatMap.empty value) d Δ σ__e ->
 
     (* [σ0] is the initial state of [d]. *)
-    Init hdstore Δ σ__e (behavior d) σ0 ->
+    Init hdstore Δ σ__e (AbstractSyntax.beh d) σ0 ->
 
     (* From [σ0] to [σ] after [↑]. *)
-    IsInjectedDState σ0 (E__p τ) σ__i ->
-    vrising hdstore Δ σ__i (behavior d) σ__r ->
-    Stabilize hdstore Δ σ__r (behavior d) σ ->
+    VConc hdstore Δ (inj σ0 (E__p τ)) rising (AbstractSyntax.beh d) σ__r ->
+    Stabilize hdstore Δ σ__r (AbstractSyntax.beh d) σ ->
     
     (* States [s] and [σ] are similar. *)
     FullSimStateAfterRE sitpn γ E__c τ (s0 sitpn) σ.
@@ -41,10 +40,10 @@ Admitted.
 #[export] Hint Extern 1 ( _ ⊢ _ ∼ _ ) => eapply first_rising_edge_full; eauto : hilecop.
 
 Lemma first_rising_edge :
-  forall sitpn id__ent id__arch b d γ E__c E__p Δ σ__e σ0 τ σ__i σ__r σ,
+  forall sitpn b d γ E__c E__p Δ σ__e σ0 τ σ__r σ,
 
     (* sitpn translates into (d, γ). *)
-    sitpn2hvhdl sitpn id__ent id__arch b = (inl (d, γ)) ->
+    sitpn2hvhdl sitpn b = (inl (d, γ)) ->
 
     (* Environments are similar. *)
     SimEnv sitpn γ E__c E__p ->
@@ -53,12 +52,12 @@ Lemma first_rising_edge :
     EDesign hdstore (NatMap.empty value) d Δ σ__e ->
 
     (* [σ0] is the initial state of [d]. *)
-    Init hdstore Δ σ__e (behavior d) σ0 ->
+    Init hdstore Δ σ__e (AbstractSyntax.beh d) σ0 ->
 
     (* From [σ0] to [σ] after [↑]. *)
-    IsInjectedDState σ0 (E__p τ) σ__i ->
-    vrising hdstore Δ σ__i (behavior d) σ__r ->
-    Stabilize hdstore Δ σ__r (behavior d) σ ->
+    VConc hdstore Δ (inj σ0 (E__p τ)) rising (AbstractSyntax.beh d) σ__r ->
+    Stabilize hdstore Δ σ__r (AbstractSyntax.beh d) σ ->
+    Stabilize hdstore Δ σ__r (AbstractSyntax.beh d) σ ->
     
     (* States [s] and [σ] are similar. *)
     SimStateAfterRE sitpn γ (s0 sitpn) σ.
