behavior-preservation/TraceSimilarity.v
@@ -22,13 +22,11 @@ Require Import hvhdl.HVhdlTypes.
 Require Import hvhdl.Environment.
 Require Import hvhdl.SemanticalDomains.
 Require Import hvhdl.Simulation.
-Require Import hvhdl.CombinationalEvaluation.
-Require Import hvhdl.SynchronousEvaluation.
 Require Import hvhdl.DesignElaboration.
 Require Import hvhdl.AbstractSyntax.
 Require Import hvhdl.HilecopDesignStore.
 Require Import hvhdl.Initialization.
-Require Import hvhdl.Stabilize.
+Require Import hvhdl.Stabilization.
 Require Import hvhdl.PortMapEvaluation.
 
 (* SITPN to H-VHDL Libraries *)
@@ -46,10 +44,10 @@ Require Import soundness.RisingEdge.
 (** ** Trace similarity lemma *)
 
 Lemma trace_sim :
-  forall sitpn id__ent id__arch b d γ E__c E__p Δ σ__e τ s σ θ__s θ__σ, 
+  forall sitpn b d γ E__c E__p Δ σ__e τ s σ θ__s θ__σ, 
 
     (* sitpn translates into (d, γ). *)
-    sitpn2hvhdl sitpn id__ent id__arch b = (inl (d, γ)) ->
+    sitpn2hvhdl sitpn b = (inl (d, γ)) ->
 
     (* Environments are similar. *)
     SimEnv sitpn γ E__c E__p ->
@@ -64,7 +62,7 @@ Lemma trace_sim :
     SitpnExecute E__c s τ θ__s ->
     
     (* From [σ], produces trace [θ__σ] after τ execution cycles. *)
-    SimLoop hdstore E__p Δ σ (behavior d) τ θ__σ ->
+    SimLoop hdstore E__p Δ σ (beh d) τ θ__σ ->
 
     (* Conclusion *)
     SimTrace γ θ__s θ__σ re.
